...

Is0/Programs.lean
@@ -59,184 +59,197 @@ def is0_constraints (input : List Felt) (output : List Felt) : Prop :=
              , output := output
              , constraints := []
              } <|
-    "1"         ←ₐ C 1;         -- %0 = cirgen.const 1
+    -- %0 = cirgen.const 1
+    "1"         ←ₐ C 1; 
     "0"         ←ₐ C 0;
-    "true"      ←ₐ ⊤;  -- %1 = cirgen.true
-    "x"         ←ₐ input[0];  -- %2 = cirgen.get %arg0[0] back 0 : <1, constant>
-    "out[0]"    ←ₐ output[0]; -- %3 = cirgen.get %arg1[0] back 0 : <2, mutable>
-    "andEqz x"  ←ₐ ⟨"true"⟩ &₀ ⟨"x"⟩; -- %4 = cirgen.and_eqz %1, %2 : <default>
-    "if out[0] then eqz x" ←ₐ guard ⟨"out[0]"⟩ & ⟨"true"⟩ with ⟨"andEqz x"⟩;  -- %5 = cirgen.and_cond %1, %3 : <default>, %4
-    "1 - out[0]" ←ₐ Op.Sub ⟨"1"⟩ ⟨"out[0]"⟩; -- %6 = cirgen.sub %0 : <default>, %3 : <default>
-    "out[1]"         ←ₐ output[1]; -- %7 = cirgen.get %arg1[1] back 0 : <2, mutable>
-    "x * out[1]"     ←ₐ Op.Mul ⟨"x"⟩ ⟨"out[1]"⟩; -- %8 = cirgen.mul %2 : <default>, %7 : <default>
-    "x * out[1] - 1" ←ₐ Op.Sub ⟨"x * out[1]"⟩ ⟨"1"⟩; -- %9 = cirgen.sub %8 : <default>, %0 : <default>
-    "other cond" ←ₐ ⟨"true"⟩ &₀ ⟨"x * out[1] - 1"⟩; -- %10 = cirgen.and_eqz %1, %9 : <default>
-    "if other cond" ←ₐ guard ⟨"1 - out[0]"⟩ & ⟨"if out[0] then eqz x"⟩ with ⟨"other cond"⟩ -- %11 = cirgen.and_cond %5, %6 : <default>, %10
-  -- (List.foldr And True) $ List.map (λ e ↦ e = 0) state'.constraints
+    -- %1 = cirgen.true
+    "true"      ←ₐ ⊤;  
+    -- %2 = cirgen.get %arg0[0] back 0 : <1, constant>
+    "x"         ←ₐ input[0];
+    -- %3 = cirgen.get %arg1[0] back 0 : <2, mutable>
+    "out[0]"    ←ₐ output[0];
+    -- %4 = cirgen.and_eqz %1, %2 : <default>
+    "andEqz x"  ←ₐ ⟨"true"⟩ &₀ ⟨"x"⟩;
+    -- %5 = cirgen.and_cond %1, %3 : <default>, %4
+    "if out[0] then eqz x" ←ₐ guard ⟨"out[0]"⟩ & ⟨"true"⟩ with ⟨"andEqz x"⟩;  
+    -- %6 = cirgen.sub %0 : <default>, %3 : <default>
+    "1 - out[0]" ←ₐ Op.Sub ⟨"1"⟩ ⟨"out[0]"⟩;
+    -- %7 = cirgen.get %arg1[1] back 0 : <2, mutable>
+    "out[1]"         ←ₐ output[1];
+    -- %8 = cirgen.mul %2 : <default>, %7 : <default>
+    "x * out[1]"     ←ₐ Op.Mul ⟨"x"⟩ ⟨"out[1]"⟩; 
+    -- %9 = cirgen.sub %8 : <default>, %0 : <default>
+    "x * out[1] - 1" ←ₐ Op.Sub ⟨"x * out[1]"⟩ ⟨"1"⟩;
+    -- %10 = cirgen.and_eqz %1, %9 : <default>
+    "other cond" ←ₐ ⟨"true"⟩ &₀ ⟨"x * out[1] - 1"⟩; 
+    -- %11 = cirgen.and_cond %5, %6 : <default>, %10
+    "if other cond" ←ₐ guard ⟨"1 - out[0]"⟩ & ⟨"if out[0] then eqz x"⟩ with ⟨"other cond"⟩ 
   (state'.props "if other cond").getD True
 
-lemma is0_constraints_closed_form {x y₁ y₂ : Felt} :
+-- lemma Map.mm {x y₁ y₂ : Felt} :
+--   ((((((Map.empty["1"] := 1)["0"] := 0)["x"] := x)["out[0]"] := y₁)["1 - out[0]"] := 1 - y₁)["out[1]"] := y₂) "1" = some 1 :=
+--     by unfold Map.update Map.empty
+--        repeat' all_goals split
+       
+lemma Map.mm {x y₁ y₂ : Felt} :
+(if "1" = "out[1]" then some y₂
+      else
+        if "1" = "1 - out[0]" then some (1 - y₁)
+        else
+          if "1" = "out[0]" then some y₁
+          else if "1" = "x" then some x else if "1" = "0" then some 0 else if "1" = "1" then some 1 else none) =
+      some 1 := by
+  repeat' split
+  all_goals try contradiction
+  rfl
+
+section tactics
+
+-- private def Map.findWith_ {β : Type} [BEq β] (keys : List String) (m : Map String β) (v : β) : α := Id.run do
+--   for key in keys do
+--     if m key = v do return 
+
+open Lean Elab Tactic
+
+elab "MLIR" : tactic => do
+  evalTactic <| ← `(
+    tactic| repeat (
+      rw [MLIR.run_Sequence_Assign_collapsible]
+      simp
+    )
+  )
+  evalTactic <| ← `(tactic| rw [MLIR.run_assign])
+  evalTactic <| ← `(tactic| simp)
+
+-- elab "MLIR_state" : tactic => do
+--   evalTactic <| ← `(
+--     tactic| repeat' split
+--   )
+--   evalTactic <| ← `(
+--     tactic| all_goals simp
+--   )
+--   evalTactic <| ← `(
+--     tactic| all_goals try contradiction
+--   )
+--   evalTactic <| ← `(
+--     tactic| all_goals try rfl
+--   )
+
+elab "MLIR_state" : tactic => do
+  evalTactic <| ← `(tactic| repeat rw [Map.update_get'])
+  evalTactic <| ← `(tactic| all_goals try decide)
+  evalTactic <| ← `(tactic| all_goals try rfl)
+  evalTactic <| ← `(tactic| all_goals simp only)
+  evalTactic <| ← `(tactic| simp)
+
+elab "MLIR_states" : tactic => do
+  evalTactic <| ← `(tactic| repeat MLIR_state)
+
+end tactics
+
+lemma is0_constraints_closed_form' {x y₁ y₂ : Felt} :
     is0_constraints [x] [y₁, y₂]
   ↔ (if 1 - y₁ = 0 then if y₁ = 0 then True else x = 0 else (if y₁ = 0 then True else x = 0) ∧ x * y₂ - 1 = 0) := by
   unfold is0_constraints
-  rw [MLIR.run_Sequence_Assign_collapsible]
-  simp only [Op.eval_getInput, List.getD_cons_zero, State.update_val]
-  rw [MLIR.run_Sequence_Assign_collapsible]
-  simp only [Op.eval_const, State.update_val]
-  rw [MLIR.run_Sequence_Assign_collapsible]
-  simp only [Op.eval_isz, Map.update_get, beq_iff_eq, ite_true, State.update_val]
-  rw [MLIR.run_Sequence_Assign_collapsible]
-  simp only [Op.eval_getInput, List.getD_cons_zero, State.update_val]
-  rw [MLIR.run_Sequence_Assign_collapsible]
-  simp only [Op.eval_getOutput, List.getD_cons_zero, State.update_val]
-  rw [MLIR.run_Sequence_Assign_collapsible]
-  simp only [Op.eval_true, State.update_constraint, List.getD_cons_zero, Op.eval_andEqz, Map.update_get, Option.some.injEq, eq_iff_iff, true_iff]
-  rw [Map.update_update_get (by decide)]
-  simp only [Option.some.injEq, forall_apply_eq_imp_iff', Op.eval.match_2.eq_2]
-  rw [MLIR.run_Sequence_Assign_collapsible]
-  simp only [
-    Op.eval_andCond, Map.update_get, beq_iff_eq, Option.some.injEq, eq_iff_iff, true_iff,
-    State.update_constraint]
-  rw [Map.update_update_get (by decide)]
-  simp only [true_and]
-  rw [MLIR.run_Sequence_Assign_collapsible]
-  simp only [Op.eval_sub, Map.update_get, Option.some.injEq, forall_apply_eq_imp_iff', State.update_val]
-  rw [Map.update_get' 1 (by simp only) _]
-  swap
-  rw [Map.update_get' 1] <;> decide
-  simp only
-  rw [MLIR.run_Sequence_Assign_collapsible]
-  simp only [Op.eval_getOutput, List.getD_cons_succ, List.getD_cons_zero, State.update_val]
-  rw [MLIR.run_Sequence_Assign_collapsible]
-  simp only [Op.eval_mul, Map.update_get, Option.some.injEq, forall_apply_eq_imp_iff', State.update_val]
-  rw [Map.update_get' x] <;> try decide
-  swap
-  rw [Map.update_get' x] <;> try decide
-  rw [Map.update_update_get (by decide)]
-  simp only
-  rw [MLIR.run_Sequence_Assign_collapsible]
-  simp only [Op.eval_sub, Map.update_get, Option.some.injEq, State.update_val]
-  rw [Map.update_get' 1] <;> try decide
-  swap
-  rw [Map.update_get' 1] <;> try decide
-  rw [Map.update_get' 1] <;> try decide
-  rw [Map.update_get' 1] <;> try decide
-  rw [Map.update_get' 1] <;> try decide
-  simp only
-  rw [MLIR.run_Sequence_Assign_collapsible]
-  simp only [Op.eval_andEqz, Map.update_get, Option.some.injEq, forall_apply_eq_imp_iff',
-  State.update_constraint]
-  rw [Map.update_get' True] <;> try decide
-  swap
-  rw [Map.update_update_get (by decide)]
-  simp only [true_and]
-  rw [MLIR.run_assign]
-  simp only [Op.eval_andCond, Map.update_get, beq_iff_eq, Option.some.injEq, eq_iff_iff,
-  State.update_constraint, Option.getD_some]
-  rw [Map.update_get' (1 - y₁)] <;> try decide
-  swap
-  rw [Map.update_get' (1 - y₁)] <;> try decide
-  rw [Map.update_get' (1 - y₁)] <;> try decide
-  simp only [Map.update_get, Option.some.injEq]
-  rw [Map.update_get' (if y₁ = 0 then True else x = 0)] <;> try decide
-  simp only [Map.update_get]
+  MLIR
+  MLIR_states
 
-lemma is0_witness_closed_form {x y₁ y₂ : Felt} :
-  is0_witness [x] = [y₁, y₂] ↔ (if x = 0 then 1 else 0) = y₁ ∧ (if x = 0 then 0 else x⁻¹) = y₂ := by
-  unfold is0_witness
-  rw [MLIR.run_Sequence_Assign_collapsible]
-  simp only [Op.eval_const, State.update_val]
-  rw [MLIR.run_Sequence_Assign_collapsible]
-  simp only [Op.eval_getInput, List.getD_cons_zero, State.update_val]
-  rw [MLIR.run_Sequence_Assign_collapsible]
-  simp only [Op.eval_isz, Map.update_get, beq_iff_eq, State.update_val]
-  rw [MLIR.run_Sequence_Set_collapsible (if x = 0 then 1 else 0)] <;> simp only [Map.update_get]
-  rw [MLIR.run_Sequence_Assign_collapsible]
-  simp only [Op.eval_inv, beq_iff_eq, State.update_val]
-  rw [Map.update_get' x (by simp only) (by simp only [Map.update_get])] ; try decide
-  simp only
-  rw [MLIR.run_Sequence_Set_collapsible (if x = 0 then 0 else x⁻¹)] <;> simp only [Map.update_get]
-  unfold List.set List.set ; simp only
-  rw [MLIR.run_Sequence_Assign_collapsible]
-  simp only [Op.eval_getOutput, List.getD_cons_zero, State.update_val]
-  rw [MLIR.run_Sequence_If_collapsible (if x = 0 then 1 else 0) (by simp only [Map.update_get])]
-  simp only [beq_iff_eq]
-  rw [MLIR.run_Sequence_Assign_collapsible]
-  simp only [Op.eval_sub, Map.update_get, Option.some.injEq, forall_apply_eq_imp_iff', State.update_val]
-  rw [Map.update_get' 1 (by simp only)] <;> try decide
-  swap
-  rw [Map.update_get' 1 (by simp only)] ; try decide
-  rw [Map.update_get' 1 (by simp only)] ; try decide
-  rw [Map.update_get' 1 (by simp only)] ; try decide
-  simp only
-  rw [MLIR.run_If_collapsible (1 - if x = 0 then 1 else 0) (by simp only [Map.update_get])]
-  rw [MLIR.run_Sequence_Assign_collapsible]
-  simp only [beq_iff_eq, Op.eval_getOutput, List.getD_cons_succ, List.getD_cons_zero, State.update_val]
-  rw [MLIR.run_Sequence_Assign_collapsible]
-  simp only [Op.eval_mul, Map.update_get, Option.some.injEq, forall_apply_eq_imp_iff', State.update_val]
-  rw [Map.update_get' x (by simp only)] <;> try decide
-  swap
-  rw [Map.update_get' x (by simp only)] ; try decide
-  rw [Map.update_get' x (by simp only)] ; try decide
-  rw [Map.update_get' x (by simp only)] ; try decide
-  rw [Map.update_get' x (by simp only)] ; try decide
-  simp only [Map.update_get]
-  simp only [mul_ite, mul_zero, ne_eq]
-  rw [MLIR.run_Sequence_Assign_collapsible]
-  simp only [Op.eval_sub, Map.update_get, Option.some.injEq, State.update_val]
-  rw [Map.update_get' 1 (by simp only)] <;> try decide
-  swap
-  rw [Map.update_get' 1 (by simp only)] ; try decide
-  rw [Map.update_get' 1 (by simp only)] ; try decide
-  rw [Map.update_get' 1 (by simp only)] ; try decide
-  rw [Map.update_get' 1 (by simp only)] ; try decide
-  rw [Map.update_get' 1 (by simp only)] ; try decide
-  rw [Map.update_get' 1 (by simp only)] ; try decide
-  simp only
-  rw [MLIR.run_Eqz_collapsible ((if x = 0 then 0 else x * x⁻¹) - 1) (by simp only [Map.update_get])]
-  simp only
-  rw [MLIR.run_Sequence_Eqz_collapsible x] <;> try simp only
-  swap
-  rw [Map.update_get' x (by simp only)] ; try decide
-  rw [Map.update_get' x (by simp only)] ; try decide
-  rw [Map.update_get' x (by simp only)] ; try decide
-  simp only [Map.update_get]
-  rw [MLIR.run_Sequence_Assign_collapsible]
-  simp only [Op.eval_sub, Map.update_get, Option.some.injEq, forall_apply_eq_imp_iff', State.update_val]
-  rw [Map.update_get' 1 (by simp only)] <;> try decide
-  swap
-  rw [Map.update_get' 1 (by simp only)] ; try decide
-  rw [Map.update_get' 1 (by simp only)] ; try decide
-  rw [Map.update_get' 1 (by simp only)] ; try decide
-  simp only
-  rw [MLIR.run_If_collapsible (1 - if x = 0 then 1 else 0) (by simp only [Map.update_get])]
-  rw [MLIR.run_Sequence_Assign_collapsible]
-  simp only [beq_iff_eq, Op.eval_getOutput, List.getD_cons_succ, List.getD_cons_zero, State.update_val]
-  rw [MLIR.run_Sequence_Assign_collapsible]
-  simp only [Op.eval_mul, Map.update_get, Option.some.injEq, forall_apply_eq_imp_iff', State.update_val]
-  rw [Map.update_get' x (by simp only)] <;> try decide
-  swap
-  rw [Map.update_get' x (by simp only)] ; try decide
-  rw [Map.update_get' x (by simp only)] ; try decide
-  rw [Map.update_get' x (by simp only)] ; try decide
-  rw [Map.update_get' x (by simp only)] ; try decide
-  simp only [Map.update_get]
-  simp only [mul_ite, mul_zero]
-  rw [MLIR.run_Sequence_Assign_collapsible]
-  simp only [Op.eval_sub, Map.update_get, Option.some.injEq, State.update_val]
-  rw [Map.update_get' 1 (by simp only)] <;> try decide
-  swap
-  rw [Map.update_get' 1 (by simp only)] ; try decide
-  rw [Map.update_get' 1 (by simp only)] ; try decide
-  rw [Map.update_get' 1 (by simp only)] ; try decide
-  rw [Map.update_get' 1 (by simp only)] ; try decide
-  rw [Map.update_get' 1 (by simp only)] ; try decide
-  rw [Map.update_get' 1 (by simp only)] ; try decide
-  simp only
-  rw [MLIR.run_Eqz_collapsible ((if x = 0 then 0 else x * x⁻¹) - 1) (by simp only [Map.update_get])]
-  rw [State.if_output]
-  rw [State.if_output]
-  rw [State.if_output]
-  simp only [ite_eq_right_iff, ite_self, List.cons.injEq, and_true]
+-- lemma is0_witness_closed_form {x y₁ y₂ : Felt} :
+--   is0_witness [x] = [y₁, y₂] ↔ (if x = 0 then 1 else 0) = y₁ ∧ (if x = 0 then 0 else x⁻¹) = y₂ := by
+--   unfold is0_witness
+--   rw [MLIR.run_Sequence_Assign_collapsible]
+--   simp only [Op.eval_const, State.update_val]
+--   rw [MLIR.run_Sequence_Assign_collapsible]
+--   simp only [Op.eval_getInput, List.getD_cons_zero, State.update_val]
+--   rw [MLIR.run_Sequence_Assign_collapsible]
+--   simp only [Op.eval_isz, Map.update_get, beq_iff_eq, State.update_val]
+--   rw [MLIR.run_Sequence_Set_collapsible (if x = 0 then 1 else 0)] <;> simp only [Map.update_get]
+--   rw [MLIR.run_Sequence_Assign_collapsible]
+--   simp only [Op.eval_inv, beq_iff_eq, State.update_val]
+--   rw [Map.update_get' x (by simp only) (by simp only [Map.update_get])] ; try decide
+--   simp only
+--   rw [MLIR.run_Sequence_Set_collapsible (if x = 0 then 0 else x⁻¹)] <;> simp only [Map.update_get]
+--   unfold List.set List.set ; simp only
+--   rw [MLIR.run_Sequence_Assign_collapsible]
+--   simp only [Op.eval_getOutput, List.getD_cons_zero, State.update_val]
+--   rw [MLIR.run_Sequence_If_collapsible (if x = 0 then 1 else 0) (by simp only [Map.update_get])]
+--   simp only [beq_iff_eq]
+--   rw [MLIR.run_Sequence_Assign_collapsible]
+--   simp only [Op.eval_sub, Map.update_get, Option.some.injEq, forall_apply_eq_imp_iff', State.update_val]
+--   rw [Map.update_get' 1 (by simp only)] <;> try decide
+--   swap
+--   rw [Map.update_get' 1 (by simp only)] ; try decide
+--   rw [Map.update_get' 1 (by simp only)] ; try decide
+--   rw [Map.update_get' 1 (by simp only)] ; try decide
+--   simp only
+--   rw [MLIR.run_If_collapsible (1 - if x = 0 then 1 else 0) (by simp only [Map.update_get])]
+--   rw [MLIR.run_Sequence_Assign_collapsible]
+--   simp only [beq_iff_eq, Op.eval_getOutput, List.getD_cons_succ, List.getD_cons_zero, State.update_val]
+--   rw [MLIR.run_Sequence_Assign_collapsible]
+--   simp only [Op.eval_mul, Map.update_get, Option.some.injEq, forall_apply_eq_imp_iff', State.update_val]
+--   rw [Map.update_get' x (by simp only)] <;> try decide
+--   swap
+--   rw [Map.update_get' x (by simp only)] ; try decide
+--   rw [Map.update_get' x (by simp only)] ; try decide
+--   rw [Map.update_get' x (by simp only)] ; try decide
+--   rw [Map.update_get' x (by simp only)] ; try decide
+--   simp only [Map.update_get]
+--   simp only [mul_ite, mul_zero, ne_eq]
+--   rw [MLIR.run_Sequence_Assign_collapsible]
+--   simp only [Op.eval_sub, Map.update_get, Option.some.injEq, State.update_val]
+--   rw [Map.update_get' 1 (by simp only)] <;> try decide
+--   swap
+--   rw [Map.update_get' 1 (by simp only)] ; try decide
+--   rw [Map.update_get' 1 (by simp only)] ; try decide
+--   rw [Map.update_get' 1 (by simp only)] ; try decide
+--   rw [Map.update_get' 1 (by simp only)] ; try decide
+--   rw [Map.update_get' 1 (by simp only)] ; try decide
+--   rw [Map.update_get' 1 (by simp only)] ; try decide
+--   simp only
+--   rw [MLIR.run_Eqz_collapsible ((if x = 0 then 0 else x * x⁻¹) - 1) (by simp only [Map.update_get])]
+--   simp only
+--   rw [MLIR.run_Sequence_Eqz_collapsible x] <;> try simp only
+--   swap
+--   rw [Map.update_get' x (by simp only)] ; try decide
+--   rw [Map.update_get' x (by simp only)] ; try decide
+--   rw [Map.update_get' x (by simp only)] ; try decide
+--   simp only [Map.update_get]
+--   rw [MLIR.run_Sequence_Assign_collapsible]
+--   simp only [Op.eval_sub, Map.update_get, Option.some.injEq, forall_apply_eq_imp_iff', State.update_val]
+--   rw [Map.update_get' 1 (by simp only)] <;> try decide
+--   swap
+--   rw [Map.update_get' 1 (by simp only)] ; try decide
+--   rw [Map.update_get' 1 (by simp only)] ; try decide
+--   rw [Map.update_get' 1 (by simp only)] ; try decide
+--   simp only
+--   rw [MLIR.run_If_collapsible (1 - if x = 0 then 1 else 0) (by simp only [Map.update_get])]
+--   rw [MLIR.run_Sequence_Assign_collapsible]
+--   simp only [beq_iff_eq, Op.eval_getOutput, List.getD_cons_succ, List.getD_cons_zero, State.update_val]
+--   rw [MLIR.run_Sequence_Assign_collapsible]
+--   simp only [Op.eval_mul, Map.update_get, Option.some.injEq, forall_apply_eq_imp_iff', State.update_val]
+--   rw [Map.update_get' x (by simp only)] <;> try decide
+--   swap
+--   rw [Map.update_get' x (by simp only)] ; try decide
+--   rw [Map.update_get' x (by simp only)] ; try decide
+--   rw [Map.update_get' x (by simp only)] ; try decide
+--   rw [Map.update_get' x (by simp only)] ; try decide
+--   simp only [Map.update_get]
+--   simp only [mul_ite, mul_zero]
+--   rw [MLIR.run_Sequence_Assign_collapsible]
+--   simp only [Op.eval_sub, Map.update_get, Option.some.injEq, State.update_val]
+--   rw [Map.update_get' 1 (by simp only)] <;> try decide
+--   swap
+--   rw [Map.update_get' 1 (by simp only)] ; try decide
+--   rw [Map.update_get' 1 (by simp only)] ; try decide
+--   rw [Map.update_get' 1 (by simp only)] ; try decide
+--   rw [Map.update_get' 1 (by simp only)] ; try decide
+--   rw [Map.update_get' 1 (by simp only)] ; try decide
+--   rw [Map.update_get' 1 (by simp only)] ; try decide
+--   simp only
+--   rw [MLIR.run_Eqz_collapsible ((if x = 0 then 0 else x * x⁻¹) - 1) (by simp only [Map.update_get])]
+--   rw [State.if_output]
+--   rw [State.if_output]
+--   rw [State.if_output]
+  -- simp only [ite_eq_right_iff, ite_self, List.cons.injEq, and_true]
 
 end Risc0
